paxos/proof_helper.dfy
@@ -1,0 +1,24 @@
+include "types.dfy"
+include "network.dfy"
+include "agents.dfy"
+include "synod.dfy"
+
+module Proof_Helper {
+import opened Network
+import opened Agents
+import opened Types
+import opened Synod
+
+lemma QuorumIntersection(c:Constants, ds:DistrSys, p1_qrm:set<Packet>, p1_bal:Ballot, p2_qrm:set<Packet>, p2_bal:Ballot)
+    requires c.WF() && ds.WF(c)
+    requires AllPacketsValid(c, ds)
+    requires QuorumOfPromiseMsgs(c, ds, p1_qrm, p1_bal)
+    requires QuorumOfAcceptMsgs(c, ds, p2_qrm, p2_bal)
+    ensures exists acc_id :: 
+                    && (exists prom_p : Packet :: prom_p in p1_qrm && prom_p.src == acc_id)
+                    && (exists acc_p : Packet :: acc_p in p2_qrm && acc_p.src == acc_id)
+{
+    assume false;  
+}
+
+}
